Clean up the ROM libraries
Now reduced to PROM as core, with ROM as a simpler interface.

PROM is concrete to allow reuse of its flag type.
Its internal theories, and ROM, are abstract to avoid growing forests of clones
when using eager arguments.

ROM now aligns with PROM in cloning interface: additional types `d_in_t` and `d_out_t`
specify the distinguisher's interface. (This simplifies instantiation.)

Some changes to type and oracle names to make them more explicit. Notably:
- `from` is now `in_t`,
- `to` is now `out_t`, (with associated change on name of distribution).

examples/hashed_elgamal_generic.ec
@@ -66,23 +66,26 @@ module Hashed_ElGamal (H:Hash): Scheme = {
   }
 }.
 
-clone import ROM.ROM_BadCall as ROC with
-  type from  <- group,
-  type to    <- bits,
-  op dsample <- fun (x:group), dbits,
-  op qH      <- qH
-proof * by exact/dbits_ll.
+clone import ROM as RO with
+  type in_t    <- group,
+  type out_t   <- bits,
+  type d_in_t  <- unit,
+  type d_out_t <- bool,
+  op   dout _  <- dbits.
+import Lazy.
+clone import ROM_BadCall as ROC with
+  op qH <- qH.
 
 (* Adversary Definitions *)
-module type Adversary (O:ARO) = {
+module type Adversary (O : POracle) = {
   proc choose(pk:pkey): ptxt * ptxt
   proc guess(c:ctxt)  : bool
 }.
 
 (* Specializing and merging the hash function *)
-module H:Hash = {
-  proc init(): unit = { RO.init(); Log.qs <- fset0; }
-  proc hash(x:group): bits = { var y; y <@ RO.o(x); return y; }
+module H : Hash = {
+  proc init(): unit = { LRO.init(); Log.qs <- fset0; }
+  proc hash(x:group): bits = { var y; y <@ LRO.o(x); return y; }
 }.
 
 (* The initial scheme *)
@@ -106,12 +109,12 @@ module SCDH_from_CPA(A:Adversary,O:Oracle): Top.SCDH.Adversary = {
 (* We want to bound the probability of A winning CPA(Bounder(A,RO),S) in terms of
    the probability of B = CDH_from_CPA(SCDH_from_CPA(A,RO)) winning CDH(B) *)
 section.
-  declare module A: Adversary {RO, Log, OnBound.G1, OnBound.G2}.
+  declare module A: Adversary { LRO, Log, OnBound.G1, OnBound.G_bad }.
 
-  axiom choose_ll (O <: ARO {A}): islossless O.o => islossless A(O).choose.
-  axiom guess_ll (O <: ARO {A}) : islossless O.o => islossless A(O).guess.
+  axiom choose_ll (O <: POracle {A}): islossless O.o => islossless A(O).choose.
+  axiom guess_ll (O <: POracle {A}) : islossless O.o => islossless A(O).guess.
 
-  local module BA = A(Bound(RO)).
+  local module BA = A(Bound(LRO)).
 
   local module G0 = {
     var gxy:group
@@ -191,7 +194,7 @@ section.
     }
   }.
 
-  local module (D : ROC.Dist) (H : ARO) = {
+  local module (D : ROC.Dist) (H : POracle) = {
     module A = A(H)
 
     var y:t
@@ -219,29 +222,29 @@ section.
     }
   }.
 
-  local lemma G0_D &m: Pr[G0.main() @ &m: res] = Pr[OnBound.G0(D,RO).main() @ &m: res].
+  local lemma G0_D &m: Pr[G0.main() @ &m: res] = Pr[OnBound.G0(D,LRO).main() @ &m: res].
   proof.
     byequiv (_: ={glob A} ==> ={res})=> //.
     proc.
-    inline OnBound.G0(D,RO).D.a1 OnBound.G0(D,RO).D.a2; wp.
+    inline D(Bound(LRO)).a1 D(Bound(LRO)).a2; wp.
     conseq (_: _ ==> ={b'} /\ b{1} = D.b{2})=> //.
     by inline H.hash; sim.
   qed.
 
-  local lemma G1_D &m: Pr[G1.main() @ &m: res] = Pr[OnBound.G1(D,RO).main() @ &m: res].
+  local lemma G1_D &m: Pr[G1.main() @ &m: res] = Pr[OnBound.G1(D,LRO).main() @ &m: res].
   proof.
     byequiv (_: ={glob A} ==> ={res})=> //.
     proc.
-    inline OnBound.G1(D,RO).D.a1 OnBound.G1(D,RO).D.a2; wp.
+    inline D(Bound(LRO)).a1 D(Bound(LRO)).a2; wp.
     conseq (_: _ ==> ={b'} /\ b{1} = D.b{2})=> //.
     by inline H.hash; sim.
   qed.
 
-  local lemma G2_D &m: Pr[G2.main() @ &m: res] = Pr[OnBound.G2(D,RO).main() @ &m: res].
+  local lemma G2_D &m: Pr[G2.main() @ &m: res] = Pr[OnBound.G_bad(D,LRO).main() @ &m: res].
   proof.
     byequiv (_: ={glob A} ==> ={res})=> //.
     proc.
-    inline OnBound.G2(D,RO).D.a1 OnBound.G2(D,RO).D.a2; wp.
+    inline D(Bound(LRO)).a1 D(Bound(LRO)).a2; wp.
     conseq (_: _ ==> ={glob Log, b'} /\ b{1} = D.b{2} /\ G2.gxy{1} = x{2})=> //.
     by inline H.hash; sim.
   qed.
@@ -249,11 +252,12 @@ section.
   local lemma G0_G1_G2 &m:
     Pr[G0.main() @ &m: res] <= Pr[G1.main() @ &m: res] + Pr[G2.main() @ &m: res].
   proof.
-    rewrite (G0_D &m) (G1_D &m) (G2_D &m).
-    apply (OnBound.ROM_BadCall D _ _ &m).
-    + move=> H0 H0_o_ll; proc; auto; call (choose_ll H0 _)=> //; auto=> />.
-      smt(dt_ll DBool.dbool_ll).
-    by progress; proc; call (guess_ll H _)=> //; auto.
+  rewrite (G0_D &m) (G1_D &m) (G2_D &m).
+  move: (OnBound.ROM_BadCall D _ _ dbits_ll &m tt true).
+  + move=> H H_o_ll; proc; auto; call (choose_ll H _)=> //; auto=> />.
+    by rewrite dt_ll DBool.dbool_ll.
+  + by move=> H H_o_ll; proc; auto; call (guess_ll H _)=> //; auto=> />.
+  by rewrite !eqT.
   qed.
 
   local module G1' = {
@@ -279,15 +283,15 @@ section.
   proof.
     byequiv (_: ={glob A} ==> ={res})=> //.
     proc.
-    call (_: ={glob RO, glob Log}); first by sim.
+    call (_: ={glob LRO, glob Log}); first by sim.
     wp; rnd (fun h, h +^ if b then m1 else m0){1}; rnd.
-    call (_: ={glob RO, glob Log}); first by sim.
-    by inline H.init RO.init; auto=> /> *; split => *; algebra.
+    call (_: ={glob LRO, glob Log}); first by sim.
+    by inline H.init LRO.init; auto=> /> *; split => *; algebra.
   qed.
 
   local lemma Pr_G1' &m: Pr[G1'.main() @ &m: res] = 1%r/2%r.
   proof.
-    cut RO_o_ll:= RO_o_ll _; first by smt(dbits_ll).
+    cut LRO_o_ll:= LRO_o_ll dbits_ll.
     byphoare (_: true ==> res)=> //.
     proc.
     swap 7 3.
@@ -295,8 +299,8 @@ section.
     conseq (_: true) => />.
     + by move=> b'; rewrite DBool.dbool1E /pred1 => />.
     islossless.
-    + by apply (guess_ll (Bound(RO))); islossless.
-    by apply (choose_ll (Bound(RO))); islossless.
+    + by apply (guess_ll (Bound(LRO))); islossless.
+    by apply (choose_ll (Bound(LRO))); islossless.
   qed.
 
   local module G2' = {
@@ -324,17 +328,17 @@ section.
   proof.
     byequiv (_: ={glob A} ==> ={res})=> //.
     proc.
-    call (_: ={glob RO, glob Log}); first by sim.
+    call (_: ={glob LRO, glob Log}); first by sim.
     wp; rnd (fun h, h +^ if b then m1 else m0){1}; rnd.
-    call (_: ={glob RO, glob Log}); first by sim.
-    by inline H.init RO.init; auto=> /> *; split => *; algebra.
+    call (_: ={glob LRO, glob Log}); first by sim.
+    by inline H.init LRO.init; auto=> /> *; split => *; algebra.
   qed.
 
-  local equiv G2'_SCDH: G2'.main ~ SCDH(SCDH_from_CPA(A,RO)).main:
+  local equiv G2'_SCDH: G2'.main ~ SCDH(SCDH_from_CPA(A,LRO)).main:
     ={glob A} ==> res{1} = res{2} /\ card Log.qs{1} <= qH.
   proof.
     proc.
-    inline SCDH_from_CPA(A,RO).solve.
+    inline SCDH_from_CPA(A,LRO).solve.
     swap{2} 5 -4; swap{1} 7 3.
     rnd{1}; wp.
     seq  8  7: (={glob BA} /\
@@ -342,23 +346,23 @@ section.
                 G2'.gxy{1} = g ^ (x * y){2} /\
                 card Log.qs{1} <= qH).
       wp; rnd; call (_: ={glob H} /\ card Log.qs{1} <= qH).
-        proc; sp; if=> //; inline Bound(RO).LO.o RO.o; auto=> />.
+        proc; sp; if=> //; inline Log(LRO).o LRO.o; auto=> />.
         by move=> &2 _ szqs_lt_qH _ _; rewrite fcardU fcard1; smt(fcard_ge0).
-      by inline H.init RO.init; auto=> />; rewrite fcards0; smt(gt0_qH pow_pow).
+      by inline H.init LRO.init; auto=> />; rewrite fcards0; smt(gt0_qH pow_pow).
     call (_: ={glob H} /\ card Log.qs{1} <= qH).
-      proc; sp; if=> //; inline Bound(RO).LO.o RO.o; auto=> /> &2 _ szqs_lt_qH _ _.
+      proc; sp; if=> //; inline Log(LRO).o LRO.o; auto=> /> &2 _ szqs_lt_qH _ _.
       by rewrite fcardU fcard1; smt(fcard_ge0).
     by auto => />.
   qed.
 
   local lemma Pr_G2'_SCDH &m :
     Pr[G2'.main() @ &m: res]
-    = Pr[SCDH(SCDH_from_CPA(A,RO)).main() @ &m : res]
+    = Pr[SCDH(SCDH_from_CPA(A,LRO)).main() @ &m : res]
   by byequiv G2'_SCDH.
 
   local lemma Reduction &m :
     Pr[CPA(S,BA).main() @ &m : res] <=
-    1%r / 2%r + Pr[SCDH(SCDH_from_CPA(A,RO)).main() @ &m : res].
+    1%r / 2%r + Pr[SCDH(SCDH_from_CPA(A,LRO)).main() @ &m : res].
   proof.
     rewrite (Pr_CPA_G0 &m).
     rewrite -(Pr_G1' &m) -(G1_G1' &m).
@@ -368,12 +372,12 @@ section.
 
   (** Composing reduction from CPA to SCDH with reduction from SCDH to CDH *)
   lemma Security &m:
-      Pr[CPA(S,A(Bound(RO))).main() @ &m: res] - 1%r / 2%r <=
-      qH%r * Pr[CDH.CDH(CDH_from_SCDH(SCDH_from_CPA(A,RO))).main() @ &m: res].
+      Pr[CPA(S,A(Bound(LRO))).main() @ &m: res] - 1%r / 2%r <=
+      qH%r * Pr[CDH.CDH(CDH_from_SCDH(SCDH_from_CPA(A,LRO))).main() @ &m: res].
   proof.
-    apply (ler_trans (Pr[SCDH(SCDH_from_CPA(A,RO)).main() @ &m: res])).
+    apply (ler_trans (Pr[SCDH(SCDH_from_CPA(A,LRO)).main() @ &m: res])).
     + smt(Reduction).
-    have:= Self.SCDH.Reduction (SCDH_from_CPA(A,RO)) &m gt0_qH.    
+    have:= Self.SCDH.Reduction (SCDH_from_CPA(A,LRO)) &m gt0_qH.    
     by rewrite -mulrA mul1r mulrC ler_pdivr_mulr 1:lt_fromint 1:gt0_qH mulrC.
   qed.
 end section.
